Update Presburger Set/PwAff definition.

Presburger.v
@@ -7,18 +7,12 @@ Require Import String.
 Local Open Scope string_scope.
 Local Open Scope Z_scope.
 
-Inductive PwAff :=
+Inductive Aff :=
 | AConst (c: Z)
 | AVar (v: string)
-| APlus (a1 a2: PwAff)
-| AMinus (a1 a2: PwAff)
-| AMul (c: Z) (a: PwAff)
-| AEq (a1 a2: PwAff)
-| ANeq (a1 a2: PwAff)
-| ALe (a1 a2: PwAff)
-| ALt (a1 a2: PwAff)
-| AGe (a1 a2: PwAff)
-| AGt (a1 a2: PwAff).
+| APlus (a1 a2: Aff)
+| AMinus (a1 a2: Aff)
+| AMul (c: Z) (a: Aff).
 
 Definition indicator (b: bool) :=
   match b with
@@ -26,78 +20,91 @@ Definition indicator (b: bool) :=
   | false => 0
   end.
 
-Fixpoint eval_aff (a: PwAff) (m: total_map Z) :=
+Fixpoint eval_aff (a: Aff) (m: total_map Z) :=
   match a with
   | AConst c => c
   | AVar v => m v
   | APlus a1 a2 => (eval_aff a1 m) + (eval_aff a2 m)
   | AMinus a1 a2 => (eval_aff a1 m) - (eval_aff a2 m)
   | AMul c a => c * (eval_aff a m)
-  | AEq a1 a2 => indicator ((eval_aff a1 m) =? (eval_aff a2 m))
-  | ANeq a1 a2 => indicator (negb ((eval_aff a1 m) =? (eval_aff a2 m)))
-  | ALe a1 a2 => indicator ((eval_aff a1 m) <=? (eval_aff a2 m))
-  | ALt a1 a2 => indicator ((eval_aff a1 m) <? (eval_aff a2 m))
-  | AGe a1 a2 => indicator ((eval_aff a1 m) >=? (eval_aff a2 m))
-  | AGt a1 a2 => indicator ((eval_aff a1 m) >? (eval_aff a2 m))
   end.
 
-Inductive Constraint :=
-| CEq (a1 a2: PwAff)
-| CNeq (a1 a2: PwAff)
-| CLe (a1 a2: PwAff)
-| CLt (a1 a2: PwAff)
-| CGe (a1 a2: PwAff)
-| CGt (a1 a2: PwAff).
-
-Definition eval_constraint (c: Constraint) (m: total_map Z) :=
-  match c with
-  | CEq a1 a2 => (eval_aff a1 m) =? (eval_aff a2 m)
-  | CNeq a1 a2 => negb ((eval_aff a1 m) =? (eval_aff a2 m))
-  | CLe a1 a2 => (eval_aff a1 m) <=? (eval_aff a2 m)
-  | CLt a1 a2 => (eval_aff a1 m) <? (eval_aff a2 m)
-  | CGe a1 a2 => (eval_aff a1 m) >=? (eval_aff a2 m)
-  | CGt a1 a2 => (eval_aff a1 m) >? (eval_aff a2 m)
-  end.
-
-Class PresburgerSet (s: Type) :=
+Class PresburgerImpl (PSet PwAff: Type) :=
   {
-    eval_set : s -> total_map Z -> bool;
+    eval_set : PSet -> total_map Z -> bool;
 
-    empty_set : s;
+    empty_set : PSet;
     empty_set_spec : forall x, eval_set empty_set x = false;
 
-    universe_set : s;
+    universe_set : PSet;
     universe_set_spec : forall x, eval_set universe_set x = true;
 
-    union_set : s -> s -> s;
+    union_set : PSet -> PSet -> PSet;
     union_set_spec : forall p1 p2 x,
         eval_set (union_set p1 p2) x = eval_set p1 x || eval_set p2 x;
 
-    intersect_set : s -> s -> s;
+    intersect_set : PSet -> PSet -> PSet;
     intersect_set_spec : forall p1 p2 x,
         eval_set (intersect_set p1 p2) x = eval_set p1 x && eval_set p2 x;
 
-    is_subset : s -> s -> bool;
+    is_subset : PSet -> PSet -> bool;
     is_subset_spec : forall p1 p2, is_subset p1 p2 = true <->
                               forall x, eval_set p1 x = true -> eval_set p2 x = true;
 
-    set_from_constraint : Constraint -> s;
-    set_from_constraint_spec : forall c x, eval_set (set_from_constraint c) x = eval_constraint c x;
-
-    set_project_out : s -> string -> s;
+    set_project_out : PSet -> string -> PSet;
     set_project_out_spec : forall p d x, eval_set (set_project_out p d) x = true <->
                                     exists v, eval_set p (d !-> v; x) = true;
+
+
+    eval_pw_aff : PwAff -> total_map Z -> option Z;
+
+    pw_aff_from_aff : Aff -> PwAff;
+    pw_aff_from_aff_spec : forall a x, eval_pw_aff (pw_aff_from_aff a) x = Some (eval_aff a x);
+
+    intersect_domain : PwAff -> PSet -> PwAff;
+    intersect_domain_spec_in : forall p s x, eval_set s x = true -> eval_pw_aff (intersect_domain p s) x = eval_pw_aff p x;
+    intersect_domain_spec_out : forall p s x, eval_set s x = false -> eval_pw_aff (intersect_domain p s) x = None;
+
+    union_pw_aff : PwAff -> PwAff -> PwAff;
+    union_pw_aff_spec : forall p1 p2 x, eval_pw_aff (union_pw_aff p1 p2) x = match eval_pw_aff p1 x with
+                                                                        | None => eval_pw_aff p2 x
+                                                                        | r => r
+                                                                        end;
+
+    eq_set : PwAff -> PwAff -> PSet;
+    eq_set_spec : forall p1 p2 x, eval_set (eq_set p1 p2) x = match (eval_pw_aff p1 x, eval_pw_aff p2 x) with
+                                                         | (Some v1, Some v2) => v1 =? v2
+                                                         | _ => false
+                                                         end;
+
+    ne_set : PwAff -> PwAff -> PSet;
+    ne_set_spec : forall p1 p2 x, eval_set (ne_set p1 p2) x = match (eval_pw_aff p1 x, eval_pw_aff p2 x) with
+                                                         | (Some v1, Some v2) => negb (v1 =? v2)
+                                                         | _ => false
+                                                         end;
+
+    le_set : PwAff -> PwAff -> PSet;
+    le_set_spec : forall p1 p2 x, eval_set (le_set p1 p2) x = match (eval_pw_aff p1 x, eval_pw_aff p2 x) with
+                                                         | (Some v1, Some v2) => v1 <=? v2
+                                                         | _ => false
+                                                         end;
+
+    indicator_function : PSet -> PwAff;
+    indicator_function_spec : forall s x, eval_pw_aff (indicator_function s) x = if eval_set s x then
+                                                                             Some 1
+                                                                         else
+                                                                           Some 0;
   }.
 
 
-Theorem is_subset_refl {s: Type} {P : PresburgerSet s} :
+Theorem is_subset_refl {PSet PwAff : Type} {P : PresburgerImpl PSet PwAff} :
   forall p, is_subset p p = true.
 Proof.
   move => p.
   apply is_subset_spec => //.
 Qed.
 
-Theorem is_subset_trans {s: Type} {P : PresburgerSet s} :
+Theorem is_subset_trans {PSet PwAff: Type} {P : PresburgerImpl PSet PwAff} :
   forall p1 p2 p3, is_subset p1 p2 = true ->
               is_subset p2 p3 = true ->
               is_subset p1 p3 = true.
@@ -107,7 +114,7 @@ Proof.
   by auto.
 Qed.
 
-Theorem is_subset_union_l {s: Type} {P: PresburgerSet s} :
+Theorem is_subset_union_l {PSet PwAff: Type} {P: PresburgerImpl PSet PwAff} :
   forall p1 p2, is_subset p1 (union_set p1 p2).
 Proof.
   move => p1 p2.
@@ -116,7 +123,7 @@ Proof.
   reflexivity.
 Qed.
 
-Theorem is_subset_union_r {s: Type} {P: PresburgerSet s} :
+Theorem is_subset_union_r {PSet PwAff: Type} {P: PresburgerImpl PSet PwAff} :
   forall p1 p2, is_subset p2 (union_set p1 p2).
 Proof.
   move => p1 p2.
@@ -125,21 +132,17 @@ Proof.
   by apply orbT.
 Qed.
 
-Theorem constraint_eq_one_variable_correct {s: Type} {P: PresburgerSet s} :
-  forall m p x, eval_set p m = eval_set (intersect_set (set_from_constraint (CEq (AVar x) (AConst (m x)))) p) m.
+Theorem constraint_eq_one_variable_correct {PSet PwAff: Type} {P: PresburgerImpl PSet PwAff} :
+  forall m p x, eval_set p m = eval_set (intersect_set (eq_set (pw_aff_from_aff (AVar x)) (pw_aff_from_aff (AConst (m x)))) p) m.
 Proof.
   move => m p x.
-  rewrite intersect_set_spec set_from_constraint_spec.
-    by rewrite /= Z.eqb_refl //.
+  by rewrite intersect_set_spec eq_set_spec !pw_aff_from_aff_spec /= Z.eqb_refl.
 Qed.
 
-Theorem constraint_neq_one_variable_correct {s: Type} {P: PresburgerSet s} :
+Theorem constraint_neq_one_variable_correct {PSet PwAff: Type} {P: PresburgerImpl PSet PwAff} :
   forall m x v, m x <> v ->
-           forall p, eval_set p m = eval_set (intersect_set (set_from_constraint (CNeq (AVar x) (AConst v))) p) m.
+           forall p, eval_set p m = eval_set (intersect_set (ne_set (pw_aff_from_aff (AVar x)) (pw_aff_from_aff (AConst v))) p) m.
 Proof.
-  move => m x v Hne p.
-  rewrite intersect_set_spec set_from_constraint_spec /=.
-  move: Hne.
-  rewrite -Z.eqb_neq => Hne.
-  rewrite Hne //.
+  move => m x v /Z.eqb_neq Hne p.
+  by rewrite intersect_set_spec ne_set_spec !pw_aff_from_aff_spec Hne.
 Qed.
